proof/crypto_scalarmult/curve25519/amd64/ref4/CorrectnessProof_ToBytes.ec
@@ -1,0 +1,791 @@
+require import Real Bool Int IntDiv List StdOrder BitEncoding.
+from Jasmin require import JModel JUtils.
+require import  Add4Extracted Sub4Extracted Mul4RefExtracted Mul4_a24RefExtracted Sqr4RefExtracted. (* must be in this order so module names do not clash *)
+require import Curve25519_Procedures Ref4_scalarmult_s CryptolineEquivs_Ref4 Zp_limbs Zp_25519 CommonCryptoline Jcheck.
+
+import Zp Ring.IntID IntOrder BS2Int.
+
+require import Array4 Array32 WArray32.
+
+(* Spec to prove smaller parts of ToBytes and then compose the, *)
+module ToBytesSpec = {
+
+ proc extract_msb(f3: W64.t) : W64.t = {
+    var _of_, _cf_, _sf_, _zf_, _0, aux_3, aux_2, aux_1, aux_0, aux : bool;
+    var aux_4: W64.t;
+
+    (aux_3, aux_2, aux_1, aux_0, aux, aux_4) <- SAR_64 f3 ((of_int 63))%W8;
+    _of_ <- aux_3;
+    _cf_ <- aux_2;
+    _sf_ <- aux_1;
+    _0 <- aux_0;
+    _zf_ <- aux;
+    f3 <- aux_4;
+    return f3;
+ }
+
+ proc remove_msb_if_set(f3: W64.t) : W64.t = {
+    var _of_, _cf_, _sf_, _zf_, _0, aux_3, aux_2, aux_1, aux_0, aux : bool;
+    var t: W64.t;
+
+    t <- LEA_64 (f3 + f3);
+    t <- t `>>` W8.one;
+
+    return t;
+ }
+
+ proc sar_inv_t (t: W64.t) : W64.t = {
+    var _of_, _cf_, _sf_, _2, _zf_ : bool;
+    var tt, tt0, tt1 : W64.t;
+
+    (_of_, _cf_, _sf_, _2, _zf_, tt) <- SAR_64 t ((of_int 63))%W8;
+    tt0 <- invw tt;
+    tt1 <- tt0 `&` (of_int 19)%W64;
+    return tt1;
+ }
+
+ proc to19(t: W64.t) : W64.t = {
+
+    t <- t `&` (of_int 19)%W64;
+    t <- t + (of_int 19)%W64;
+
+    return t;
+ }
+
+ proc addition(f: Rep4, operand2: W64.t) : Rep4 = {
+  var aux_4, tt, tt0 : W64.t;
+  var _of_, _cf_, _sf_, _zf_, cf, _0, _1, _2, aux_3 : bool;
+  var ff : Rep4; (* we don't change the value of f, easier proofs *)
+  tt <- f.[3];
+
+  (aux_3, aux_4) <- addc f.[0] operand2 false;
+  cf <- aux_3;
+  ff <- ff.[0 <- aux_4];
+  (aux_3, aux_4) <- addc f.[1] W64.zero cf;
+  cf <- aux_3;
+  ff <- ff.[1 <- aux_4];
+  (aux_3, aux_4) <- addc f.[2] W64.zero cf;
+  cf <- aux_3;
+  ff <- ff.[2 <- aux_4];
+  (_1, tt0) <- addc tt W64.zero cf;
+  ff <- ff.[3 <- tt0];
+
+  return ff;
+ }
+
+ proc subtraction(f: Rep4, operand2: W64.t) : Rep4 = {
+  var aux_4 : W64.t;
+  var _of_, _cf_, _sf_, _zf_, cf, _0, _1, _2, _3, aux_3 : bool;
+  var ff : Rep4; (* we don't change the value of f, easier proofs *)
+
+
+  (aux_3, aux_4) <- subc f.[0] operand2 false;
+  cf <- aux_3;
+  ff <- ff.[0 <- aux_4];
+  (aux_3, aux_4) <- subc f.[1] W64.zero cf;
+  cf <- aux_3;
+  ff <- ff.[1 <- aux_4];
+  (aux_3, aux_4) <- subc f.[2] W64.zero cf;
+  cf <- aux_3;
+  ff <- ff.[2 <- aux_4];
+  (aux_3, aux_4) <- subc f.[3] W64.zero cf;
+  _3 <- aux_3;
+  ff <- ff.[3 <- aux_4];
+
+  return ff;
+ }
+
+ (* We show that for 0 <= valrep4 f < 2^255, the first three calls essentially do nothing *)
+ proc addition_calls(f: Rep4) : Rep4 = {
+   var tt, tt0, extracted_msbw : W64.t;
+   var ff : Rep4; (* we don't change the value of f, easier proofs *)
+   ff <- witness;
+   extracted_msbw <@ extract_msb (f.[3]);
+   tt  <@ remove_msb_if_set (f.[3]);
+   tt0 <@ to19 (extracted_msbw);
+   ff <@ addition(f, tt0);
+   return ff;
+ }
+
+ proc tobytes_no_reduction(f: Rep4) : Rep4 = {
+     var tt, tt0, f3, extracted_msbw : W64.t;
+     var ff, ff2: Rep4; (* we don't change the value of f, easier proofs *)
+
+     ff <@ addition_calls(f);              (* ff = f + 19 *)
+     f3 <@ sar_inv_t(ff.[3]);              (* f3 = 19 *)
+     ff2  <@ subtraction(ff, f3);          (* ff2 = ff - 19 = f + 19 - 19 = f *)
+     return ff2;
+ }
+
+
+}.
+
+(* Helper lemmas *)
+lemma cminusP0 r: 0 <= r < p => r = asint (inzp r).
+proof. move => H. rewrite inzpK pE => />. rewrite modz_small. apply bound_abs. smt(pVal). auto. qed.
+
+lemma cminusP1 r: p <= r < 2*p => r - p = asint (inzp r).
+proof. rewrite inzpK => />. move => [#] H H0. smt(pE pVal). qed.
+
+lemma cminusP2 r: 2*p <= r < W256.modulus => r - p - p = asint (inzp r).
+proof. rewrite inzpK => />. move => [#] H H0. smt(pE pVal). qed.
+
+lemma upper_limb4_lt_2_255_range r: 0 <= valRep4 r < pow 2 255 => 0 <= (to_uint r.[3]) < pow 2 63.
+proof. rewrite valRep4E /to_list /val_digits /mkseq -iotaredE => />. smt(W64.to_uint_cmp). qed.
+
+lemma upper_limb4_ltP_range r: 0 <= valRep4 r < p => 0 <= (to_uint r.[3]) < pow 2 63.
+proof. rewrite valRep4E pE /to_list /val_digits /mkseq -iotaredE => />. smt(W64.to_uint_cmp). qed.
+
+lemma upper_limb4_ltP_msb r: 0 <= valRep4 r < p => r.[3].[63] = false.
+proof. move => H. have E: b2i r.[3].[63] = 0.
+       rewrite b2i_get //=. move: upper_limb4_ltP_range W64.to_uint_cmp; 1:smt(). smt(). qed.
+
+lemma upper_limb4_ltP_msbw r: 0 <=  W64.to_uint r < pow 2 63 => r.[63] = false.
+proof. move => H. have E: b2i r.[63] = 0.
+       rewrite b2i_get //=. move: H. smt(). smt(). qed.
+
+lemma upper_limb4_geq_2_255_range r: pow 2 255 <= valRep4 r < W256.modulus =>
+           pow 2 63 <= (to_uint r.[3]) < W64.modulus.
+proof. rewrite valRep4E /to_list /val_digits /mkseq -iotaredE => />.
+       move => H H0. do split. move: W64.to_uint_cmp. smt(). move: W64.to_uint_cmp. smt(). qed.
+
+lemma upper_limb4_p_2_255_range r: p <= valRep4 r < pow 2 255 =>
+           pow 2 63 - 1 <= (to_uint r.[3]) < W64.modulus.
+proof. rewrite valRep4E pE /to_list /val_digits /mkseq -iotaredE => />.
+       move => H H0. do split. move: W64.to_uint_cmp. smt(). move: W64.to_uint_cmp. smt(). qed.
+
+lemma upper_limb4_geqP_range r: p <= valRep4 r < W256.modulus =>
+           (pow 2 63) - 1 <= (to_uint r.[3]) < W64.modulus.
+proof. rewrite valRep4E pE /to_list /val_digits /mkseq -iotaredE => />.
+       move => H H0. do split. move: W64.to_uint_cmp. smt(). move: W64.to_uint_cmp. smt(). qed.
+
+lemma upper_limb4_geq_2_255_msb r: pow 2 255 <= valRep4 r < W256.modulus => r.[3].[63] = true.
+proof. move => H. have E: b2i r.[3].[63] = 1.
+       rewrite b2i_get //=. move: H upper_limb4_geq_2_255_range W64.to_uint_cmp; 1:smt(). smt(). qed.
+
+lemma upper_limb4_geqP_msbw r: pow 2 63  <=  W64.to_uint r < W64.modulus => r.[63] = true.
+proof. move => H. have E: b2i r.[63] = 1.
+       rewrite b2i_get //=. move: H upper_limb4_geq_2_255_range W64.to_uint_cmp; 1:smt(). smt(). qed.
+
+lemma helper_remove_msb_if_set (f: W64.t):
+    0 <= W64.to_uint f < pow 2 63 => LEA_64 (f + f) `>>` W8.one = f.
+proof.
+    auto => />. rewrite /LEA_64 => *.
+    have E: W64.to_uint (f + f `>>` W8.of_int 1) = W64.to_uint f.
+    rewrite to_uint_shr //= !to_uintD !modz_small /absz //=.
+    smt(). smt(). smt(@W64).
+qed.
+
+lemma helper_sar_inv_t (t: W64.t) : 0 <= u64i t && u64i t < pow 2 63 => invw (SAR_64 t ((of_int 63))%W8).`6 `&` (of_int 19)%W64 = (of_int 19)%W64.
+proof.
+    auto => />. move => H H0.
+    have ->: (SAR_64 t ((of_int 63))%W8).`6 = W64.zerow.
+    + rewrite /SAR_64 /shift_mask /rflags_OF //= sarE /min => />.
+    rewrite init_bits2w bits2wE -iotaredE /min //=.
+    rewrite upper_limb4_ltP_msbw //=.
+    + rewrite /W64.zerow /W64.zero bits2wE /int2bs /mkseq -iotaredE => />.
+    have ->: invw W64.zerow = W64.onew.
+    + rewrite /invw mapE /W64.zerow /W64.zero bits2wE /int2bs /mkseq -iotaredE => />.
+    + rewrite /W64.onew of_intE bits2wE /int2bs /mkseq -iotaredE => />.
+    + rewrite wordP => i ib. rewrite !initiE 1,2:/# //= initiE 1:/# //= 1:/#.
+    rewrite wordP => i ib.
+    rewrite /W64.onew !of_intE !bits2wE !/int2bs !/mkseq -!iotaredE => />.
+    rewrite !initiE 1,2:/# //= /#.
+qed.
+
+lemma not_false_to_true bst: (bst <> false) = (bst = true) by smt().
+
+
+(** Lossless lemmas **)
+
+lemma ill_sar_inv_t: islossless ToBytesSpec.sar_inv_t by proc; wp; skip => />.
+lemma ill_remove_msb_if_set_lt_2_255: islossless ToBytesSpec.remove_msb_if_set by proc; wp; skip => />.
+lemma ill_extract_msb_lt_2_255: islossless ToBytesSpec.extract_msb by proc; wp; skip => />.
+lemma ill_to19: islossless ToBytesSpec.to19 by proc; wp; skip => />.
+lemma ill_addition: islossless ToBytesSpec.addition by proc; wp; skip => />.
+lemma ill_subtraction: islossless ToBytesSpec.subtraction by proc; wp; skip => />.
+
+(** Case: 0 <= valRep4 f < p (some lemmas can be till < 2 255) **)
+
+(** SAR+INV+AND **)
+lemma h_sar_inv_t:
+  hoare [ToBytesSpec.sar_inv_t :
+      0 <= W64.to_uint t < pow 2 63
+      ==>
+      res = W64.of_int 19].
+    proc => />. auto => />.
+    move => &h H H0. rewrite helper_sar_inv_t. smt(). auto.
+qed.
+
+lemma ph_sar_inv_t:
+  phoare [ToBytesSpec.sar_inv_t :
+      0 <= W64.to_uint t < pow 2 63
+      ==>
+      res = W64.of_int 19] = 1%r.
+proof.
+    by conseq ill_sar_inv_t (h_sar_inv_t).
+qed.
+
+(** Remove MSB if it is set **)
+lemma h_remove_msb_if_set_lt_2_255 (r: W64.t):
+  hoare [ToBytesSpec.remove_msb_if_set :
+      r = f3 /\ 0 <= W64.to_uint r < pow 2 63
+      ==>
+      r = res
+  ].
+    proc => />. wp; skip => />. move => *.
+    rewrite helper_remove_msb_if_set /#.
+qed.
+
+lemma ph_remove_msb_if_set_lt_2_255 (r: W64.t):
+  phoare [ToBytesSpec.remove_msb_if_set :
+      r = f3 /\ 0 <= W64.to_uint r < pow 2 63
+      ==>
+      r = res] = 1%r.
+proof.
+    by conseq ill_remove_msb_if_set_lt_2_255 (h_remove_msb_if_set_lt_2_255 r).
+qed.
+
+(** Extracts MSB **)
+lemma h_extract_msb_lt_2_255:
+  hoare [ToBytesSpec.extract_msb :
+      0 <= W64.to_uint f3 < pow 2 63
+      ==>
+      res = W64.zerow
+  ].
+    proc => />. wp; skip => /> &hr H H0.
+    rewrite /SAR_64 /shift_mask /rflags_OF //= sarE.
+    rewrite init_bits2w bits2wE -iotaredE /min //=.
+    rewrite upper_limb4_ltP_msbw //=.
+    + rewrite /W64.zerow /W64.zero bits2wE /int2bs /mkseq -iotaredE => />.
+qed.
+
+lemma ph_extract_msb_lt_2_255:
+  phoare [ToBytesSpec.extract_msb :
+      0 <= W64.to_uint f3 < pow 2 63
+      ==>
+      res = W64.zerow] = 1%r.
+proof.
+    by conseq ill_extract_msb_lt_2_255 (h_extract_msb_lt_2_255).
+qed.
+
+(** Sets word to 19 if word = 0 **)
+lemma h_to19:
+  hoare [ToBytesSpec.to19 :
+      t = W64.zerow
+      ==>
+      res = W64.of_int 19
+  ].
+    proc => />. wp; skip => /> &hr H H0.
+qed.
+
+
+lemma ph_to19:
+  phoare [ToBytesSpec.to19 :
+      t = W64.zerow
+      ==>
+      res = W64.of_int 19] = 1%r.
+proof.
+    by conseq ill_to19 (h_to19).
+qed.
+
+(** Adding 19 to a Rep4 **)
+
+abbrev add19_l1 (r: Rep4) = (addc r.[0] ((of_int 19))%W64 false).`2.
+abbrev add19_l2 (r: Rep4) = (addc r.[1] W64.zero (addc_carry r.[0] ((of_int 19))%W64 false)).`2.
+abbrev add19_l3 (r: Rep4) = (addc r.[2] W64.zero (addc_carry r.[1] W64.zero (addc_carry r.[0] ((of_int 19))%W64 false))).`2.
+abbrev add19_l4 (r: Rep4) = (addc r.[3] W64.zero (addc_carry r.[2] W64.zero (addc_carry r.[1] W64.zero (addc_carry r.[0] ((of_int 19))%W64 false)))).`2.
+
+abbrev add19 (r: Rep4) = Array4.of_list witness [add19_l1 r; add19_l2 r ; add19_l3 r ; add19_l4 r].
+
+lemma h_addition19 (r: Rep4):
+  hoare [ToBytesSpec.addition :
+      r = f /\ operand2 = W64.of_int 19 /\  0 <= valRep4 r < p
+      ==>
+      res = add19 r /\ valRep4 r + 19 = valRep4 res
+  ].
+proof.
+    proc. auto => />. move => &hr H H0. do split.
+    + apply Array4.ext_eq => i ib. rewrite !addcE. rewrite !get_setE 1..4:/#.
+    + case(i = 3) => C. rewrite C => />.
+    + case(i = 2) => C0. rewrite C0 => />.
+    + case(i = 1) => C1. rewrite C1 => />.
+    + case(i = 0) => C2. rewrite C2 => />. smt().
+    rewrite !addcE !/add_carry !/carry_add !b2i0 => />.
+    rewrite !valRep4E !/to_list !/val_digits !/mkseq -!iotaredE => />.
+    rewrite !mulzDr -!mulzA !to_uintD !of_uintK (modz_small 19 (pow 2 64)) 1:/# => />.
+    case((18446744073709551616 <= u64i r.[0] + 19) = false) => C1. rewrite C1 !b2i0 => />.
+    + rewrite pmod_small. move: C1 W64.to_uint_cmp. smt().
+    + rewrite pmod_small. move: W64.to_uint_cmp. smt().
+    + rewrite pmod_small. move: W64.to_uint_cmp. smt().
+    + rewrite pmod_small. move: W64.to_uint_cmp. smt().
+    + have ->: (18446744073709551616 <= u64i r.[1] = false). move: W64.to_uint_cmp => />. smt().
+    + have ->: (18446744073709551616 <= u64i r.[2] = false). move: W64.to_uint_cmp => />. smt().
+    + rewrite pmod_small. move: W64.to_uint_cmp. smt(). ring.
+
+    move: C1. rewrite not_false_to_true. move => C1. rewrite !C1 !b2i1.
+    case(18446744073709551616 <= u64i r.[1] + 1 = false) => C2. rewrite !C2 !b2i0.
+    + rewrite (pmod_small (u64i r.[1] + 1 %% 18446744073709551616) 18446744073709551616).
+    + move :W64.to_uint_cmp. smt(). auto => />.
+    + rewrite (pmod_small (u64i r.[2]) 18446744073709551616). move: C1 W64.to_uint_cmp. smt().
+    + have ->: (u64i r.[0] + 19) %% 18446744073709551616 = (u64i r.[0] + 19) - 18446744073709551616.
+    + move :W64.to_uint_cmp. smt(). move: W64.to_uint_cmp. smt().
+
+    move: C2. rewrite not_false_to_true. move => C2. rewrite !C2 !b2i1.
+    + rewrite (pmod_small 1 18446744073709551616). auto => />.
+    + have ->: (u64i r.[1] + 1) %% 18446744073709551616 = (u64i r.[1] + 1) - 18446744073709551616.
+    + move: W64.to_uint_cmp. smt().
+    + have ->: (u64i r.[0] + 19) %% 18446744073709551616 = (u64i r.[0] + 19) - 18446744073709551616.
+    + move: W64.to_uint_cmp. smt().
+
+    case(18446744073709551616 <= u64i r.[2] + 1 = false) => C3. rewrite C3 b2i0 => />.
+    + rewrite pmod_small. move: W64.to_uint_cmp. smt().
+    + rewrite pmod_small. move: W64.to_uint_cmp. smt(). ring.
+
+    move: C3. rewrite not_false_to_true. move => C3. rewrite !C3 !b2i1 => />.
+    + have ->: (u64i r.[2] + 1) %% 18446744073709551616 = (u64i r.[2] + 1) - 18446744073709551616.
+    + move: W64.to_uint_cmp. smt().
+    + have E: 0 <= u64i r.[3] && u64i r.[3] < pow 2 63.
+    + apply upper_limb4_ltP_range. smt().
+    + rewrite pmod_small. move: E. smt().
+    ring.
+qed.
+
+lemma ph_addition19 (r: Rep4):
+  phoare [ToBytesSpec.addition :
+      r = f /\ operand2 = W64.of_int 19 /\  0 <= valRep4 r < p
+      ==>
+      res = add19 r /\ valRep4 r + 19 = valRep4 res
+  ] = 1%r.
+proof.
+    by conseq ill_addition (h_addition19 r).
+qed.
+
+lemma h_addition19_calls (r: Rep4):
+  equiv [ToBytesSpec.addition_calls ~ ToBytesSpec.addition :
+      0 <= valRep4 f{1} < p /\ ={f} /\ operand2{2} = W64.of_int 19
+      ==>
+       valRep4 res{1} = valRep4 res{2}
+  ].
+proof.
+    proc *. auto => />. inline {1} 1.
+    seq 3 0 : (#pre /\ f0{1} = f{2} /\ ff{1} = witness /\ extracted_msbw{1} = W64.zerow).
+    + ecall {1} (ph_extract_msb_lt_2_255). auto => />.
+    + move => &2 H H0.
+    + move: upper_limb4_ltP_range r. smt().
+    seq 1 0 : (#pre /\ tt{1} = f0{1}.[3]).
+    + ecall {1} (ph_remove_msb_if_set_lt_2_255 (f0{1}.[3])).
+    + auto => />. move => &1 &2 [#] H. do split.
+    + move: (upper_limb4_ltP_range (f{1})) (W64.to_uint_cmp f{1}.[3]). auto => />.
+    + move: (upper_limb4_ltP_range (f{1})) (W64.to_uint_cmp f{1}.[3]). auto => />. smt().
+    seq 1 0 : (#pre /\ tt0{1} = W64.of_int 19).
+    + ecall {1} (ph_to19). auto => />. wp.
+    ecall {1} (ph_addition19 (f0{1})).
+    ecall {2} (ph_addition19 (f{2})).
+    auto => />.
+qed.
+
+(** Substraction **)
+lemma h_subtraction19 (r: Rep4):
+  hoare [ToBytesSpec.subtraction :
+      r = f /\ operand2 = W64.of_int 19 /\ 19 <= valRep4 r < W256.modulus
+      ==>
+      valRep4 r - 19 = valRep4 res
+  ].
+proof.
+    proc. auto => />. move => &hr H H0.
+    rewrite !subcE !/borrow_sub !b2i0 => />.
+    rewrite !valRep4E !/to_list !/val_digits !/mkseq -!iotaredE => />.
+    rewrite !mulzDr -!mulzA !to_uintD !to_uintN (modz_small 19 (pow 2 64)) 1:/# => />.
+
+    case ((u64i r.[0] < 19) = false) => C1. rewrite !C1 !b2i0 !to_uint0 => />.
+    have ->: u64i r.[1] < 0 = false. move: W64.to_uint_cmp; 1:smt().
+    have ->: u64i r.[2] < 0 = false. move: W64.to_uint_cmp; 1:smt().
+    rewrite !b2i0 => />.
+    + have ->: (u64i r.[0] + 18446744073709551597) %% 18446744073709551616 =
+               (u64i r.[0] + 18446744073709551597) - 18446744073709551616.
+    + move: W64.to_uint_cmp. smt(). auto => />.
+    + rewrite pmod_small. move: W64.to_uint_cmp. smt().
+    + rewrite pmod_small. move: W64.to_uint_cmp. smt().
+    + rewrite pmod_small. move: W64.to_uint_cmp. smt().
+    + ring.
+
+    move: C1. rewrite not_false_to_true. move => C1. rewrite !C1 !b2i1 !to_uint1 => />.
+    rewrite pmod_small. move: W64.to_uint_cmp. smt().
+    case ((u64i r.[1] < 1) = false) => C2. rewrite !C2 !b2i0 !to_uint0 => />.
+    + have ->: u64i r.[2] < 0 = false. move: W64.to_uint_cmp; 1:smt().
+    + rewrite !b2i0 => />.
+    + have ->: (u64i r.[1] + 18446744073709551615) %% 18446744073709551616 =
+               (u64i r.[1] + 18446744073709551615) - 18446744073709551616.
+    + move: W64.to_uint_cmp. smt(). auto => />.
+    + rewrite pmod_small. move: W64.to_uint_cmp. smt().
+    + rewrite pmod_small. move: W64.to_uint_cmp. smt().
+    + ring.
+
+    move: C2. rewrite not_false_to_true. move => C2. rewrite !C2 !b2i1 !to_uint1 => />.
+    rewrite pmod_small. move: W64.to_uint_cmp. smt().
+    case ((u64i r.[2] < 1) = false) => C3. rewrite !C3 !b2i0 !to_uint0 => />.
+    + have ->: (u64i r.[2] + 18446744073709551615) %% 18446744073709551616 =
+               (u64i r.[2] + 18446744073709551615) - 18446744073709551616.
+    + move: W64.to_uint_cmp. smt(). auto => />.
+    + rewrite pmod_small. move: W64.to_uint_cmp. smt().
+    + ring.
+
+    move: C3. rewrite not_false_to_true. move => C3. rewrite !C3 !b2i1 !to_uint1 => />.
+    rewrite pmod_small. move: W64.to_uint_cmp. smt().
+    have E: ((u64i r.[3] < 1) = false).
+    + move: (W64.to_uint_cmp r.[3])  (upper_limb4_ltP_range r) H H0.
+    + rewrite !valRep4E !pE !/to_list !/val_digits !/mkseq -!iotaredE => />.
+    + rewrite !mulzDr -!mulzA   (modz_small 0 (pow 2 64)) 1:/# => />; 1:smt().
+    + have ->: (u64i r.[3] + 18446744073709551615) %% 18446744073709551616 =
+               (u64i r.[3] + 18446744073709551615) - 18446744073709551616.
+    + move: W64.to_uint_cmp. smt(). auto => />. ring.
+qed.
+
+lemma ph_subtraction19 (r: Rep4):
+  phoare [ToBytesSpec.subtraction :
+       r = f /\ operand2 = W64.of_int 19 /\ 19 <= valRep4 r < W256.modulus
+      ==>
+      valRep4 r - 19 = valRep4 res
+  ] = 1%r.
+proof.
+    by conseq ill_subtraction (h_subtraction19 r).
+qed.
+
+(** To Bytes **)
+lemma h_tobytes_no_reduction (r: Rep4):
+  hoare [ToBytesSpec.tobytes_no_reduction :
+      r = f /\ 0 <= valRep4 r < p
+      ==>
+      valRep4 r = valRep4 res
+  ].
+proof.
+    proc. inline 1.
+    seq 3 : (#pre /\ extracted_msbw0 = W64.zerow /\ f0 = f).
+    + call h_extract_msb_lt_2_255. auto => />.
+    + move => H H0. move: (upper_limb4_ltP_range r). smt().
+    seq 1 : (#pre /\ tt1 = f.[3]).
+    + call (h_remove_msb_if_set_lt_2_255 (r.[3])). auto => />.
+    + move: (upper_limb4_ltP_range r). smt().
+    seq 1 : (#pre /\ tt00 = W64.of_int 19).
+    + call h_to19. auto => />.
+    + seq 1 : (#pre /\ valRep4 r + 19 = valRep4 ff0 /\ add19 r = ff0).
+    + call (h_addition19 r). auto => />.
+    seq 2 : (#pre /\ f3 = W64.of_int 19 /\ ff = ff0).
+    + call h_sar_inv_t. auto => />.
+    + move => &hr.
+    rewrite !addcE !/add_carry !/carry_add !b2i0 => />.
+    rewrite !valRep4E !pVal !/to_list !/val_digits !/mkseq -!iotaredE => />.
+    rewrite !mulzDr -!mulzA !to_uintD !of_uintK (modz_small 19 (pow 2 64)) 1:/# => />.
+    + move: (upper_limb4_ltP_range r).
+    + move: (W64.to_uint_cmp (add19_l4 r)). smt().
+    call (h_subtraction19 (add19 r)). auto => />.
+    move => &hr [#] H H0. do split;1:smt(). move: H.
+    rewrite pVal 1:/#. smt().
+qed.
+
+lemma equiv_to_bytes_no_reduction:
+    equiv[M.__tobytes4 ~ ToBytesSpec.tobytes_no_reduction :
+      f{1} = f{2} /\ 0 <= valRep4 f{1} < p
+      ==>
+      valRep4 res{1} = valRep4 res{2}
+    ].
+proof.
+    proc => />.
+    inline {2} 1. swap {2} 4 -1. swap{1} 9 -7.
+    seq 2 3: (#pre /\ t{1} = tt1{2} /\ tt1{2} = f0.[3]{2} /\ 0 <= valRep4 f0{2} < p /\ f0{2} = f{2}).
+    + wp; sp. ecall {2} (ph_remove_msb_if_set_lt_2_255 f0.[3]{2}). auto => />.
+    + move => &2 [#] H H0. do split. smt(W64.to_uint_cmp).
+    + move: H H0 upper_limb4_lt_2_255_range W64.to_uint_cmp pVal; 1:smt().
+    + move => H1 H2. rewrite helper_remove_msb_if_set /#.
+
+    seq 6 1 : (#pre /\ extracted_msbw0{2} = W64.zerow /\ aux_4{1} = extracted_msbw0{2}).
+    + auto => />.
+    + ecall {2} (ph_extract_msb_lt_2_255). auto => />.
+    + move => &2 H H0 H1 H2. do split. smt(W64.to_uint_cmp).
+    + move: H1 H2. rewrite valRep4E pE /to_list /val_digits /mkseq -iotaredE => />.
+    + smt(W64.to_uint_cmp). move => H3 H4.
+    + rewrite /SAR_64 /shift_mask /rflags_OF //= sarE /min => />.
+    + rewrite init_bits2w bits2wE -iotaredE /min //= upper_limb4_ltP_msbw.
+    + move: H H0. rewrite valRep4E pE /to_list /val_digits /mkseq -iotaredE => />.
+    + rewrite /W64.zerow of_intE bits2wE /int2bs /mkseq -iotaredE => />.
+
+    seq 1 0 : (0 <= valRep4 f{1} && valRep4 f{1} < p - W64.to_uint (f.[3]{2}) /\ t{1} = tt1{2}
+               /\ tt1{2} = f0{2}.[3] /\
+               0 <= valRep4 f0{2} && valRep4 f0{2} < p /\ extracted_msbw0{2} = W64.zerow /\
+               aux_4{1} = extracted_msbw0{2} /\ f0{2} = f{2} /\
+               f{1} = Array4.of_list witness [f.[0]{2}; f.[1]{2}; f.[2]{2}; extracted_msbw0{2}]).
+    + auto => />. move => &2 H H0 H1 H2. do split.
+    + rewrite valRep4E /to_list /val_digits /mkseq -iotaredE => />. smt(W64.to_uint_cmp).
+    + move => H3. do split.
+    + move: H H0. rewrite !valRep4E !pE !/to_list !/val_digits !/mkseq -!iotaredE => />.
+    + rewrite to_uint0 => />. smt(W64.to_uint_cmp). apply Array4.ext_eq => i ib.
+    + rewrite !get_setE 1:/#.
+    + case (i = 3) => I. rewrite I => />.
+    + case (i = 2) => I0. rewrite I0 => />.
+    + case (i = 1) => I1. rewrite I1 => />.
+    + case (i = 0) => I2. rewrite I2 => />. rewrite get_out /#.
+
+    seq 2 1 : (0 <= valRep4 f{1} && valRep4 f{1} < p - (W64.to_uint f.[3]{2}) + 19 * pow 2 196 /\
+               t{1} = tt1{2} /\ tt1{2} = f0{2}.[3] /\ 0 <= valRep4 f0{2} && valRep4 f0{2} < p
+               /\ extracted_msbw0{2} = W64.zerow /\ f0{2} = f{2}
+               /\ tt00{2} = W64.of_int 19 /\ f.[0]{1} = f.[0]{2} /\ f.[1]{1} = f.[1]{2} /\
+               f.[2]{1} = f.[2]{2} /\  f.[3]{1} = tt00{2}).
+   + ecall {2} (ph_to19). wp. auto => />. move => &2 [#] H H0 H1 H2. do split.
+   + move: H. rewrite !valRep4E !/to_list !/val_digits !/mkseq -!iotaredE => />.
+   + rewrite to_uint0 => />. smt(W64.to_uint_cmp). move => H3.
+   + have !->: W64.zerow `&` (of_int 19)%W64 + (of_int 19)%W64 = W64.of_int 19. smt(@W64).
+   + move: H0. rewrite !valRep4E pE !/to_list !/val_digits !/mkseq -!iotaredE => />. rewrite to_uint0 //=.
+   + smt(W64.to_uint_cmp).
+
+   seq 0 0 : (#pre /\ f{1} = Array4.of_list witness [f.[0]{2}; f.[1]{2}; f.[2]{2}; tt00{2}]).
+   + skip. move => &1 &2 [#] H H0 H1 H2 H3 H4 H5 H6 H7 H8 H9 H10.
+   + auto => />. move => *. auto => />. rewrite -H8 -H9 -H10 H7.
+   + apply Array4.ext_eq => i ib.
+    + case (i = 3) => I. rewrite I => />.
+    + case (i = 2) => I0. rewrite I0 => />.
+    + case (i = 1) => I1. rewrite I1 => />.
+    + case (i = 0) => I2. rewrite I2 => />. rewrite get_out /#.
+
+    seq 10 1 : (0 <= valRep4 f0{2} && valRep4 f0{2} < p
+               /\ extracted_msbw0{2} = W64.zerow /\ f0{2} = f{2}
+               /\ tt00{2} = W64.of_int 19 /\ 19 <= valRep4 ff0{2} && valRep4 ff0{2} < p+19 /\
+               ff0{2} = add19 f0{2} /\ f{1}.[0] = add19_l1 f{2} /\ f{1}.[1] = add19_l2 f{2} /\
+               f{1}.[2] = add19_l3 f{2} /\ f{1}.[3] = W64.of_int 19 /\ t{1} = add19_l4 f0{2}
+               /\ t{1} = add19_l4 f{2}).
+   + ecall {2} (ph_addition19 f0{2}). auto => />. move => &1 [#] H H0 H1 H2 H3.
+   + do split. rewrite -H3 1:/#. move => H4.  rewrite -H3 1:/#.
+
+   seq 0 1 : (#pre /\ ff{2} = ff0{2}). auto => />.
+
+   swap{1} 3 -1.
+   seq 2 0 : (ff{2} = ff0{2} /\ 0 <= valRep4 f0{2} && valRep4 f0{2} < p /\ t{1} = add19_l4 f{2} /\
+               0 <= valRep4 f{1} && valRep4 f{1} < p + 19
+               /\ extracted_msbw0{2} = W64.zerow /\ f0{2} = f{2}
+               /\ tt00{2} = W64.of_int 19 /\ 19 <= valRep4 ff0{2} && valRep4 ff0{2} < p+19 /\
+               ff0{2} = add19 f0{2} /\ f{1}.[0] = add19_l1 f{2} /\ f{1}.[1] = add19_l2 f{2} /\
+               f{1}.[2] = add19_l3 f{2} /\ f{1}.[3] = ff0.[3]{2}).
+   + auto => />. move => &1 &2 [#] H H0 H1 H2 H3 H4 H5 H6. do split.
+   + rewrite valRep4E /to_list /val_digits /mkseq -iotaredE => />. smt(W64.to_uint_cmp). move => H7.
+   + do split. move: H2. rewrite !valRep4E !pVal !/to_list !/val_digits !/mkseq -!iotaredE => />.
+   + have ->: LEA_64 (add19_l4 f{2} + add19_l4 f{2}) `>>` W8.one = add19_l4 f{2}.
+   + rewrite helper_remove_msb_if_set. move: H0.
+   + rewrite !valRep4E !pVal !/to_list !/val_digits !/mkseq -!iotaredE => />.
+   + rewrite !addcE !/carry_add !b2i0 => />.
+   + case (18446744073709551616 <= u64i f{2}.[0] + 19 = false) => C. rewrite !C !b2i0 => />.
+   + have !->: 18446744073709551616 <= u64i f{2}.[1] = false. move: W64.to_uint_cmp. smt().
+   + have !->: 18446744073709551616 <= u64i f{2}.[2] = false. move: W64.to_uint_cmp. smt().
+   + rewrite !b2i0 => />. smt(W64.to_uint_cmp).
+   + move: C. rewrite not_false_to_true. move => C. rewrite !C !b2i1 => />.
+   + case (18446744073709551616 <= u64i f{2}.[1] + 1 = false) => C1. rewrite !C1 !b2i0 => />.
+   + have !->: 18446744073709551616 <= u64i f{2}.[2] = false. move: W64.to_uint_cmp. smt().
+   + rewrite !b2i0 => />. smt(W64.to_uint_cmp).
+   + move: C1. rewrite not_false_to_true. move => C1. rewrite !C1 !b2i1 => />.
+   + case (18446744073709551616 <= u64i f{2}.[2] + 1 = false) => C2. rewrite !C2 !b2i0 => />.
+   + smt(W64.to_uint_cmp).
+   + move: C2. rewrite not_false_to_true. move => C2. rewrite !C2 !b2i1 => />.
+   + rewrite !to_uintD of_uintK. smt(W64.to_uint_cmp).
+   + auto => />. move => H8. smt().
+   + have ->: LEA_64 (add19_l4 f{2} + add19_l4 f{2}) `>>` W8.one = add19_l4 f{2}.
+   + rewrite helper_remove_msb_if_set. move: H0.
+   + rewrite !valRep4E !pVal !/to_list !/val_digits !/mkseq -!iotaredE => />.
+   + rewrite !addcE !/carry_add !b2i0 => />.
+   + case (18446744073709551616 <= u64i f{2}.[0] + 19 = false) => C. rewrite !C !b2i0 => />.
+   + have !->: 18446744073709551616 <= u64i f{2}.[1] = false. move: W64.to_uint_cmp. smt().
+   + have !->: 18446744073709551616 <= u64i f{2}.[2] = false. move: W64.to_uint_cmp. smt().
+   + rewrite !b2i0 => />. smt(W64.to_uint_cmp).
+   + move: C. rewrite not_false_to_true. move => C. rewrite !C !b2i1 => />.
+   + case (18446744073709551616 <= u64i f{2}.[1] + 1 = false) => C1. rewrite !C1 !b2i0 => />.
+   + have !->: 18446744073709551616 <= u64i f{2}.[2] = false. move: W64.to_uint_cmp. smt().
+   + rewrite !b2i0 => />. smt(W64.to_uint_cmp).
+   + move: C1. rewrite not_false_to_true. move => C1. rewrite !C1 !b2i1 => />.
+   + case (18446744073709551616 <= u64i f{2}.[2] + 1 = false) => C2. rewrite !C2 !b2i0 => />.
+   + smt(W64.to_uint_cmp).
+   + move: C2. rewrite not_false_to_true. move => C2. rewrite !C2 !b2i1 => />.
+   + rewrite !to_uintD of_uintK. smt(W64.to_uint_cmp). auto => />. auto => />.
+
+   seq 3 1 : (ff{2} = ff0{2} /\ 0 <= valRep4 f0{2} && valRep4 f0{2} < p /\
+               0 <= valRep4 f{1} && valRep4 f{1} < p + 19
+               /\ extracted_msbw0{2} = W64.zerow /\ f0{2} = f{2}
+               /\ tt00{2} = W64.of_int 19 /\ 19 <= valRep4 ff0{2} && valRep4 ff0{2} < p+19 /\
+               ff0{2} = add19 f0{2} /\ f{1}.[0] = add19_l1 f{2} /\ f{1}.[1] = add19_l2 f{2} /\
+               f{1}.[2] = add19_l3 f{2} /\ f{1}.[3] = ff0.[3]{2} /\ f3{2} = W64.of_int 19 /\
+               t{1} = W64.of_int 19).
+   + ecall {2} (ph_sar_inv_t). auto => />. move => &1 &2 [#] H H0 H1 H2 H3 H4 H5 H6 H7 H8.
+   + do split. smt(W64.to_uint_cmp). move: H4.
+   + rewrite !valRep4E !pVal !/to_list !/val_digits !/mkseq -!iotaredE => />.
+   + rewrite !addcE !/carry_add !b2i0 => />.
+   + case (18446744073709551616 <= u64i f{2}.[0] + 19 = false) => C. rewrite !C !b2i0 => />.
+   + have !->: 18446744073709551616 <= u64i f{2}.[1] = false. move: W64.to_uint_cmp. smt().
+   + have !->: 18446744073709551616 <= u64i f{2}.[2] = false. move: W64.to_uint_cmp. smt().
+   + rewrite !b2i0 => />. smt(W64.to_uint_cmp).
+   + move: C. rewrite not_false_to_true. move => C. rewrite !C !b2i1 => />.
+   + case (18446744073709551616 <= u64i f{2}.[1] + 1 = false) => C1. rewrite !C1 !b2i0 => />.
+   + have !->: 18446744073709551616 <= u64i f{2}.[2] = false. move: W64.to_uint_cmp. smt().
+   + rewrite !b2i0 => />. smt(W64.to_uint_cmp).
+   + move: C1. rewrite not_false_to_true. move => C1. rewrite !C1 !b2i1 => />.
+   + case (18446744073709551616 <= u64i f{2}.[2] + 1 = false) => C2. rewrite !C2 !b2i0 => />.
+   + smt(W64.to_uint_cmp).
+   + move: C2. rewrite not_false_to_true. move => C2. rewrite !C2 !b2i1 => />.
+   + rewrite !to_uintD of_uintK. smt(W64.to_uint_cmp).
+   + auto => />. move => H9 H10.
+   + rewrite helper_sar_inv_t 1:/#. auto.
+   ecall {2} (ph_subtraction19 ff{2}). auto => />.
+   + move => &1 &2 H H0 H1 H2 H3 H4 H5 H6 H7 H8. do split.
+   + move: H4. rewrite !valRep4E !pVal !/to_list !/val_digits !/mkseq -!iotaredE => />.
+   + rewrite !addcE !/carry_add !b2i0 => />.
+   + case (18446744073709551616 <= u64i f{2}.[0] + 19 = false) => C. rewrite !C !b2i0 => />.
+   + have !->: 18446744073709551616 <= u64i f{2}.[1] = false. move: W64.to_uint_cmp. smt().
+   + have !->: 18446744073709551616 <= u64i f{2}.[2] = false. move: W64.to_uint_cmp. smt().
+   + rewrite !b2i0 => />. smt(W64.to_uint_cmp).
+   + move: C. rewrite not_false_to_true. move => C. rewrite !C !b2i1 => />.
+   + case (18446744073709551616 <= u64i f{2}.[1] + 1 = false) => C1. rewrite !C1 !b2i0 => />.
+   + have !->: 18446744073709551616 <= u64i f{2}.[2] = false. move: W64.to_uint_cmp. smt().
+   + rewrite !b2i0 => />. smt(W64.to_uint_cmp).
+   + move: C1. rewrite not_false_to_true. move => C1. rewrite !C1 !b2i1 => />.
+   + case (18446744073709551616 <= u64i f{2}.[2] + 1 = false) => C2. rewrite !C2 !b2i0 => />.
+   + smt(W64.to_uint_cmp).
+   + move: C2. rewrite not_false_to_true. move => C2. rewrite !C2 !b2i1 => />.
+   + rewrite !to_uintD of_uintK. smt(W64.to_uint_cmp).
+   + move => H9 H10 H11. rewrite -H11 H5 H6 H7 H8.
+   + rewrite !addcE !/carry_add !b2i0 => />.
+   + rewrite !subcE !/borrow_sub !b2i0 => />.
+   + rewrite !valRep4E !/to_list !/val_digits !/mkseq -!iotaredE => />.
+   + rewrite !mulzDr -!mulzA !to_uintD !to_uintN (modz_small 19 (pow 2 64)) 1:/# => />.
+   + rewrite !of_uintK => />.
+   + case (18446744073709551616 <= u64i f{2}.[0] + 19 = false) => C. rewrite !C !b2i0 => />.
+   + have ->: (18446744073709551616 <= u64i f{2}.[1] = false). move: W64.to_uint_cmp => />. smt().
+   + have ->: (18446744073709551616 <= u64i f{2}.[2] = false). move: W64.to_uint_cmp => />. smt().
+   + rewrite (pmod_small (u64i f{2}.[3]) 18446744073709551616). move: W64.to_uint_cmp => />. smt().
+   + rewrite (pmod_small (u64i f{2}.[2]) 18446744073709551616). move: W64.to_uint_cmp => />. smt().
+   + rewrite (pmod_small (u64i f{2}.[1]) 18446744073709551616). move: W64.to_uint_cmp => />. smt().
+   + rewrite (pmod_small (u64i f{2}.[0] + 19) 18446744073709551616). move: W64.to_uint_cmp => />. smt().
+   + have ->: u64i f{2}.[0] + 19 < 19 = false. move: W64.to_uint_cmp => />. smt().
+   + have ->: u64i f{2}.[1] < 0 = false. move: W64.to_uint_cmp => />. smt().
+   + have ->: u64i f{2}.[2] < 0 = false. move: W64.to_uint_cmp => />. smt().
+   + rewrite !b2i0 => />.
+   + rewrite (pmod_small (u64i f{2}.[3]) 18446744073709551616). move: W64.to_uint_cmp => />. smt().
+   + rewrite (pmod_small (u64i f{2}.[2]) 18446744073709551616). move: W64.to_uint_cmp => />. smt().
+   + rewrite (pmod_small (u64i f{2}.[1]) 18446744073709551616). move: W64.to_uint_cmp => />. smt().
+   + have ->: (u64i f{2}.[0] + 18446744073709551616) %% 18446744073709551616 = (u64i f{2}.[0] + 18446744073709551616) - 18446744073709551616. move: W64.to_uint_cmp. smt().
+   + ring.
+
+   move: C. rewrite not_false_to_true. move => C. rewrite !C !b2i1.
+   case(18446744073709551616 <= u64i f{2}.[1] + 1 = false) => C1. rewrite !C1 !b2i0 => />.
+   + have ->: (18446744073709551616 <= u64i f{2}.[2] = false). move: W64.to_uint_cmp => />. smt().
+   + rewrite (pmod_small (u64i f{2}.[3]) 18446744073709551616). move: W64.to_uint_cmp => />. smt().
+   + rewrite (pmod_small (u64i f{2}.[2]) 18446744073709551616). move: W64.to_uint_cmp => />. smt().
+   + have ->: ((u64i f{2}.[0] + 19) %% 18446744073709551616 < 19) = true. move: W64.to_uint_cmp => />. smt().
+   + have ->: ((u64i f{2}.[1] + 1) %% 18446744073709551616 < 1) = false. move: W64.to_uint_cmp => />. smt().
+   + have ->: ((u64i f{2}.[2] < 0)) = false. move: W64.to_uint_cmp => />. smt().
+   + rewrite !b2i0 !b2i1 => />.
+   + rewrite (pmod_small (u64i f{2}.[3]) 18446744073709551616). move: W64.to_uint_cmp => />. smt().
+   + rewrite (pmod_small (u64i f{2}.[2]) 18446744073709551616). move: W64.to_uint_cmp => />. smt().
+   + have ->: (u64i f{2}.[0] + 19) %% 18446744073709551616 = (u64i f{2}.[0] + 19) - 18446744073709551616. move: W64.to_uint_cmp => />. smt().
+   + rewrite (pmod_small (u64i f{2}.[1] + 1) 18446744073709551616). move: W64.to_uint_cmp => />. smt().
+   + have ->: (u64i f{2}.[1] + 1 + 18446744073709551615) %% 18446744073709551616 = (u64i f{2}.[1] + 1 + 18446744073709551615) - 18446744073709551616. move: W64.to_uint_cmp => />. smt(). auto => />.
+   + rewrite (pmod_small (u64i f{2}.[0]) 18446744073709551616). move: W64.to_uint_cmp => />. smt().
+   + ring.
+
+   move: C1. rewrite not_false_to_true. move => C1. rewrite !C1 !b2i1.
+   case(18446744073709551616 <= u64i f{2}.[2] + 1 = false) => C2. rewrite !C2 !b2i0 => />.
+   + rewrite (pmod_small (u64i f{2}.[3]) 18446744073709551616). move: W64.to_uint_cmp => />. smt().
+   + have ->: ((u64i f{2}.[0] + 19) %% 18446744073709551616 < 19) = true. move: W64.to_uint_cmp => />. smt().
+   + have ->: ((u64i f{2}.[1] + 1) %% 18446744073709551616 < 1) = true. move: W64.to_uint_cmp => />. smt().
+   + rewrite  !b2i1 => />.
+   + have ->: (u64i f{2}.[0] + 19) %% 18446744073709551616 = (u64i f{2}.[0] + 19) - 18446744073709551616. move: W64.to_uint_cmp => />. smt().
+   + have ->: (u64i f{2}.[2] + 1) %% 18446744073709551616 < 1 = false. move: W64.to_uint_cmp => />. smt().
+   + rewrite (pmod_small (u64i f{2}.[0]) 18446744073709551616). move: W64.to_uint_cmp => />. smt().
+   + rewrite (pmod_small (u64i f{2}.[2] + 1) 18446744073709551616). move: W64.to_uint_cmp => />. smt().
+   + have ->: (u64i f{2}.[2] + 1 + 18446744073709551615) %% 18446744073709551616 = (u64i f{2}.[2] + 1 + 18446744073709551615) - 18446744073709551616. move: W64.to_uint_cmp => />. smt(). auto => />.
+   + have ->: (u64i f{2}.[1] + 1) %% 18446744073709551616 = (u64i f{2}.[1] + 1 - 18446744073709551616). move: W64.to_uint_cmp => />. smt(). rewrite !b2i0 => />.
+   + rewrite (pmod_small (u64i f{2}.[3]) 18446744073709551616). move: W64.to_uint_cmp => />. smt().
+   + rewrite (pmod_small (u64i f{2}.[1]) 18446744073709551616). move: W64.to_uint_cmp => />. smt().
+   + ring.
+
+   move: C2. rewrite not_false_to_true. move => C2. rewrite !C2 !b2i1.
+   have E: (18446744073709551616 <= u64i f{2}.[3] + 1 = false).
+   + move: (W64.to_uint_cmp f{2}.[3])  (upper_limb4_ltP_range f{2}) H H0 H1 H2 H3 H4 H9.
+   + rewrite !valRep4E !pE !/to_list !/val_digits !/mkseq -!iotaredE => />.
+   + rewrite !mulzDr -!mulzA   (modz_small 0 (pow 2 64)) 1:/# => />; 1:smt().
+
+   + have ->: ((u64i f{2}.[0] + 19) %% 18446744073709551616 < 19) = true. move: W64.to_uint_cmp => />. smt().
+   + have ->: ((u64i f{2}.[1] + 1) %% 18446744073709551616 < 1) = true. move: W64.to_uint_cmp => />. smt().
+   + rewrite  !b2i1 => />.
+   + have !->: (u64i f{2}.[0] + 19) %% 18446744073709551616 = (u64i f{2}.[0] + 19) - 18446744073709551616. move: W64.to_uint_cmp => />. smt().
+   + have ->: (u64i f{2}.[2] + 1) %% 18446744073709551616 < 1 = true. move: W64.to_uint_cmp => />. smt().
+   + rewrite (pmod_small (u64i f{2}.[0]) 18446744073709551616). move: W64.to_uint_cmp => />. smt().
+   + have !->: (u64i f{2}.[2] + 1) %% 18446744073709551616 = (u64i f{2}.[2] + 1) - 18446744073709551616. move: W64.to_uint_cmp => />. smt(). auto => />.
+   + have !->: (u64i f{2}.[1] + 1) %% 18446744073709551616 = (u64i f{2}.[1] + 1) - 18446744073709551616. move: W64.to_uint_cmp => />. smt(). auto => />.
+   + rewrite pmod_small. move: W64.to_uint_cmp => />. smt().
+   + rewrite pmod_small. move: W64.to_uint_cmp => />. smt().
+   + rewrite !b2i1 => />.
+   + rewrite (pmod_small (u64i f{2}.[3] + 1) 18446744073709551616). move: W64.to_uint_cmp => />. smt().
+   + have !->: (u64i f{2}.[3] + 1 + 18446744073709551615) %% 18446744073709551616 = (u64i f{2}.[3] + 1 + 18446744073709551615) - 18446744073709551616. move: W64.to_uint_cmp => />. smt().
+   + ring.
+qed.
+
+(** Case p <= valRep4 < 2*p (some lemmas extend to 2**256)**)
+
+lemma h_sar_inv_t_of:
+  hoare [ToBytesSpec.sar_inv_t :
+      pow 2 63 <= W64.to_uint t < W64.modulus
+      ==>
+      res = W64.zerow].
+    proc => />. auto => />.
+    move => &hr H H0.
+    have ->: (SAR_64 t{hr} ((of_int 63))%W8).`6 = W64.onew.
+    + rewrite /SAR_64 /shift_mask /rflags_OF //= sarE /min => />.
+    rewrite init_bits2w bits2wE -iotaredE /min //= upper_limb4_geqP_msbw.
+    move: H upper_limb4_geq_2_255_range W64.to_uint_cmp; 1:smt().
+    + rewrite /W64.onew of_intE bits2wE /int2bs /mkseq -iotaredE => />.
+    have ->: invw W64.onew = W64.zerow.
+    + rewrite /invw mapE /W64.zerow /W64.zero bits2wE /int2bs /mkseq -iotaredE => />.
+    + rewrite wordP => i ib. rewrite !initiE 1,2,3:/# //=.
+    rewrite wordP => i ib.
+    rewrite /W64.zerow /W64.zero !bits2wE !/int2bs !/mkseq -!iotaredE => />.
+    rewrite !initiE 1,2:/# //= /#.
+qed.
+
+lemma ph_sar_inv_t_of:
+  phoare [ToBytesSpec.sar_inv_t :
+      pow 2 63 <= W64.to_uint t < W64.modulus
+      ==>
+      res = W64.zerow] = 1%r.
+proof.
+    by conseq ill_sar_inv_t (h_sar_inv_t_of).
+qed.
+
+(** Subtraction **)
+
+lemma h_subtraction0 (r: Rep4):
+  hoare [ToBytesSpec.subtraction :
+      r = f /\ operand2 = W64.of_int 0
+      ==>
+      valRep4 r = valRep4 res
+  ].
+proof.
+    proc. auto => />. move => &hr.
+    rewrite !subcE !/borrow_sub !b2i0 => />.
+    rewrite !valRep4E !/to_list !/val_digits !/mkseq -!iotaredE => />.
+    rewrite !mulzDr -!mulzA !to_uintD !to_uintN (modz_small 0 (pow 2 64)) 1:/# => />.
+    have ->: u64i r.[0] < 0 = false. move: W64.to_uint_cmp; 1:smt().
+    have ->: u64i r.[1] < 0 = false. move: W64.to_uint_cmp; 1:smt().
+    have ->: u64i r.[2] < 0 = false. move: W64.to_uint_cmp; 1:smt().
+    rewrite pmod_small. move: W64.to_uint_cmp; 1:smt().
+    rewrite !b2i0 => />.
+    rewrite pmod_small. move: W64.to_uint_cmp; 1:smt().
+    rewrite pmod_small. move: W64.to_uint_cmp; 1:smt().
+    rewrite pmod_small. move: W64.to_uint_cmp; 1:smt().
+    auto.
+qed.
+
+lemma ph_subtraction0 (r: Rep4):
+  phoare [ToBytesSpec.subtraction :
+      r = f /\ operand2 = W64.of_int 0
+      ==>
+      valRep4 r = valRep4 res
+  ] = 1%r.
+proof.
+    by conseq ill_subtraction (h_subtraction0 r).
+qed.
